Smt/Preprocess/NegateGoal.lean
@@ -1,0 +1,24 @@
+/-
+Copyright (c) 2021-2026 by the authors listed in the file AUTHORS and their
+institutional affiliations. All rights reserved.
+Released under Apache 2.0 license as described in the file LICENSE.
+Authors: Abdalrhman Mohamed
+-/
+
+import Smt.Preprocess.Basic
+import Lean.Meta.Tactic.Apply
+import Lean.Meta.Tactic.Intro
+
+namespace Smt.Preprocess
+
+open Lean
+
+def negateGoal (mv : MVarId) (hs : Array Expr) : MetaM Result := do
+  let target ← mv.getType
+  if target.isFalse then return { map := {}, hs, mv }
+  let [mv] ← mv.applyConst ``Classical.byContradiction
+    | throwError "[negateGoal] Unexpected result after applying {``Classical.byContradiction}"
+  let (fv, mv) ← mv.intro1
+  return { map := Std.HashMap.insert {} (.fvar fv) #[.fvar fv], hs := hs.push (.fvar fv), mv }
+
+end Smt.Preprocess
