Test/Int/Let.lean
@@ -3,10 +3,12 @@ import Smt
 variable (f : Int → Int)
 
 example (h : f 10 = 10) : let y := 10; f y = 10 := by
-  smt [h]
+  -- smt -intros [h] -- TODO: why is there a PANIC?
+  smt +mono [h]
 
 example (h : let y := 10; f y = 10) : f 10 = 10 := by
-  smt [h]
+  -- smt -intros [h] -- TODO: why is there a PANIC?
+  smt +mono [h]
 
 example (h : f 10 = 10) : f 10 = 10 := by
   let z : Int := 10
